deps/poulet4/lib/LightTyping/ValueTyping.v
@@ -2,6 +2,30 @@ Require Export Poulet4.Semantics Poulet4.LightTyping.Utility
         Poulet4.Value Coq.micromega.Lia Poulet4.Utils
         Poulet4.Monads.Monad Poulet4.Monads.Option.
 
+Lemma split_inj : forall (U V : Type) (uvs₁ uvs₂ : list (U * V)),
+    split uvs₁ = split uvs₂ -> uvs₁ = uvs₂.
+Proof.
+  intros U V usv1;
+    induction usv1 as [| [u1 v1] usv1 IHusv1];
+    intros [| [u2 v2] usv2] H;
+    simpl in *; auto.
+  - destruct (split usv2) as [us2 vs2] eqn:H2; inversion H.
+  - destruct (split usv1) as [us1 vs1] eqn:H1; inversion H.
+  - specialize IHusv1 with usv2.
+    destruct (split usv1) as [us1 vs1] eqn:H1;
+      destruct (split usv2) as [us2 vs2] eqn:H2.
+    inversion H; subst; f_equal; auto.
+Qed.
+
+Lemma map_pat_combine : forall (T U V W: Type) (f : T -> V) (g : U -> W) tus,
+    map (fun '(t,u) => (f t, g u)) tus =
+    combine (map f (map fst tus)) (map g (map snd tus)).
+Proof.
+  intros T U V W f g tus;
+    induction tus as [| [t u] tus IHtus];
+    simpl; f_equal; auto.
+Qed.
+
 (** Predicate that a
     [read_one_bit] relation
     is productive. *)
@@ -56,9 +80,6 @@ Section ValueTyping.
     | typ_tuple : forall vs ts,
         Forall2 val_typ vs ts ->
         val_typ (ValBaseTuple vs) (TypTuple ts)
-    | typ_record : forall vs ts,
-        AList.all_values val_typ vs (P4String.clear_AList_tags ts) ->
-        val_typ (ValBaseRecord vs) (TypRecord ts)
     | typ_error : forall err,
         val_typ (ValBaseError err) TypError
     | typ_matchkind : forall mk,
@@ -108,10 +129,6 @@ Section ValueTyping.
           Forall2 val_typ vs ts ->
           Forall2 P vs ts ->
           P (ValBaseTuple vs) (TypTuple ts).
-      Hypothesis HRecord : forall vs ts,
-          AList.all_values val_typ vs (P4String.clear_AList_tags ts) ->
-          AList.all_values P vs (P4String.clear_AList_tags ts) ->
-          P (ValBaseRecord vs) (TypRecord ts).
       Hypothesis HError : forall err,
           P (ValBaseError err) TypError.
       Hypothesis HMatchkind : forall mk,
@@ -185,8 +202,6 @@ Section ValueTyping.
           | typ_varbit _ _ H => HVarbit _ _ H
           | typ_string s => HString s
           | typ_tuple _ _ H => HTuple _ _ H (lind H)
-          | typ_record _ _ H =>
-            HRecord _ _ H (alind H)
           | typ_error err => HError err
           | typ_matchkind mk => HMatchkind mk
           | typ_struct _ _ H => HStruct _ _ H (alind H)
@@ -227,18 +242,6 @@ Section ValueTyping.
             by (rewrite map_length; reflexivity); auto.
         - constructor; rewrite map_length; auto.
         - rewrite Forall2_map_l in H0; auto.
-        - constructor.
-          unfold AList.all_values in *.
-          rewrite Forall2_conj in *;
-            destruct H0 as [Hnames Hvts]; split.
-          + clear Hvts.
-            rewrite Forall2_map_both in *.
-            rewrite map_fst_map, map_id.
-            assumption.
-          + clear Hnames.
-            rewrite Forall2_map_both, map_snd_map,
-            map_map, <- Forall2_map_both.
-            assumption.
         - constructor.
           unfold AList.all_values in *.
           rewrite Forall2_conj in *;
@@ -333,18 +336,6 @@ Section ValueTyping.
         - constructor.
           unfold AList.all_values in *.
           rewrite Forall2_conj in *.
-          destruct H0 as [Habkeys Habtyps].
-          destruct H2 as [Hakeys Hatyps].
-          rewrite Forall2_map_both in *.
-          pose proof Forall2_map_both
-               _ _ _ _ (fun va vb => forall t, val_typ gsa va t -> val_typ gsb vb t)
-               snd snd kvas kvbs as H';
-            cbn in *; apply H' in Habtyps; clear H'.
-          rewrite Forall2_eq in *; rewrite <- Habkeys.
-          rewrite Forall2_map_both; split; eauto.
-        - constructor.
-          unfold AList.all_values in *.
-          rewrite Forall2_conj in *.
           destruct H1 as [Habkeys Habtyps].
           destruct H5 as [Hakeys Hatyps].
           rewrite Forall2_map_both in *.
@@ -418,20 +409,6 @@ Section ValueTyping.
           firstorder eauto.
         - rewrite Forall_snd, Forall_exists_factor in H.
           destruct H as [bs Hbs].
-          exists (ValBaseRecord (combine (map fst vs) bs)).
-          constructor. unfold AList.all_values.
-          rewrite Forall2_conj.
-          split; rewrite Forall2_map_both.
-          + rewrite Forall2_eq.
-            rewrite map_fst_combine;
-              autorewrite with core; eauto.
-          + rewrite Forall2_map_l in Hbs.
-            rewrite map_snd_combine;
-              autorewrite with core; eauto.
-            apply Forall2_length in Hbs.
-            autorewrite with core in *; assumption.
-        - rewrite Forall_snd, Forall_exists_factor in H.
-          destruct H as [bs Hbs].
           exists (ValBaseStruct (combine (map fst vs) bs)).
           constructor. unfold AList.all_values.
           rewrite Forall2_conj.
@@ -482,16 +459,155 @@ Section ValueTyping.
   End RelTyp.
 
   Section Uninit.
+    Fixpoint normᵗ (t : typ) : typ :=
+      match t with
+      | TypBool
+      | TypString
+      | TypInteger
+      | TypInt _
+      | TypBit _
+      | TypVarBit _
+      | TypError
+      | TypMatchKind
+      | TypVoid
+      | TypTypeName _
+      | TypExtern _
+      | TypTable _   => t
+      | TypArray t n => TypArray (normᵗ t) n
+      | TypList  ts
+      | TypTuple ts  => TypTuple (map normᵗ ts)
+      | TypRecord ts
+      | TypStruct ts => TypStruct (map (fun '(x,t) => (x, normᵗ t)) ts)
+      | TypSet    t  => TypSet (normᵗ t)
+      | TypHeader ts => TypHeader (map (fun '(x,t) => (x, normᵗ t)) ts)
+      | TypHeaderUnion ts => TypHeaderUnion (map (fun '(x,t) => (x, normᵗ t)) ts)
+      | TypEnum X t ms    => TypEnum X (option_map normᵗ t) ms
+      | TypNewType _ t    => normᵗ t
+      | TypControl ct             => TypControl (normᶜ ct)
+      | TypParser  ct             => TypParser  (normᶜ ct)
+      | TypFunction ft            => TypFunction (normᶠ ft)
+      | TypAction cs ds           => TypAction (map normᵖ cs) (map normᵖ ds)
+      | TypPackage Xs ws ps       => TypPackage Xs ws (map normᵖ ps)
+      | TypSpecializedType t ts   => TypSpecializedType (normᵗ t) (map normᵗ ts)
+      | TypConstructor Xs ws ps t => TypConstructor Xs ws (map normᵖ ps) (normᵗ t)
+      end
+    with normᶜ (ct : ControlType) : ControlType :=
+           match ct with
+           | MkControlType Xs ps => MkControlType Xs (map normᵖ ps)
+           end
+    with normᶠ (ft : FunctionType) : FunctionType :=
+           match ft with
+           | MkFunctionType Xs ps k t
+             => MkFunctionType Xs (map normᵖ ps) k (normᵗ t)
+           end
+    with normᵖ (p : P4Parameter) : P4Parameter :=
+           match p with
+           | MkParameter b d t a x => MkParameter b d (normᵗ t) a x
+           end.
+
+    Definition normᵗ_idem_def t := normᵗ (normᵗ t) = normᵗ t.
+    Definition normᶜ_idem_def t := normᶜ (normᶜ t) = normᶜ t.
+    Definition normᶠ_idem_def t := normᶠ (normᶠ t) = normᶠ t.
+    Definition normᵖ_idem_def t := normᵖ (normᵖ t) = normᵖ t.
+
+    Definition normᵗ_idem_ind :=
+      my_P4Type_ind
+        _ normᵗ_idem_def normᶜ_idem_def
+        normᶠ_idem_def normᵖ_idem_def.
+
+    Ltac list_idem :=
+      intros ts Hts; f_equal;
+      apply map_ext_Forall in Hts;
+      rewrite map_map; auto; assumption.
+    
+    Ltac alist_idem :=
+      intros xts Hxts; f_equal;
+      pose proof Forall_map
+           (fun t => normᵗ (normᵗ t) = normᵗ t) snd xts
+        as H; unfold Basics.compose in H;
+      rewrite <- H in Hxts; clear H;
+      apply map_ext_Forall in Hxts;
+      repeat rewrite map_pat_combine;
+      repeat rewrite map_fst_combine;
+      repeat rewrite map_snd_combine;
+      repeat rewrite map_length; auto;
+      repeat rewrite map_id; rewrite map_map;
+      f_equal; auto; assumption.
+    
+    Lemma normᵗ_idem : forall t, normᵗ_idem_def t.
+    Proof.
+      apply normᵗ_idem_ind;
+        unfold normᵗ_idem_def,normᶜ_idem_def,
+        normᶠ_idem_def,normᵖ_idem_def; cbn in *;
+          try (intros; f_equal; eauto; assumption);
+          try list_idem; try alist_idem; eauto.
+      - intros X [t |] ms H; inversion H; subst; cbn; do 2 f_equal; auto.
+      - intros ds cs Hds Hcs.
+        apply map_ext_Forall in Hds, Hcs.
+        repeat rewrite map_map; f_equal; auto.
+      - intros Xs ws ps H.
+        apply map_ext_Forall in H.
+        repeat rewrite map_map; f_equal; auto.
+      - intros t ts Hts Ht.
+        apply map_ext_Forall in Hts;
+          rewrite map_map; f_equal; auto.
+      - intros Xs ws ps t Hps Ht.
+        apply map_ext_Forall in Hps;
+          rewrite map_map; f_equal; auto.
+      - intros Xs ps Hps;
+          apply map_ext_Forall in Hps;
+          rewrite map_map; f_equal; auto.
+      - intros Xs ps k t Hps Ht;
+          apply map_ext_Forall in Hps;
+          rewrite map_map; f_equal; auto.
+    Qed.
+    
     Context {dummy : Inhabitant tags_t}.
 
-    Definition uninit_sval_of_typ_val_typ_def (t : typ) :=
-      forall b v ge, uninit_sval_of_typ b t = Some v -> val_typ ge v t.
+    Definition uninit_sval_of_typ_norm_def t :=
+      forall b, uninit_sval_of_typ b (normᵗ t) = uninit_sval_of_typ b t.
 
-    Definition uninit_sval_of_typ_val_typ_ind :=
+    Definition uninit_sval_of_typ_norm_ind :=
       my_P4Type_ind
-        _ uninit_sval_of_typ_val_typ_def
+        _ uninit_sval_of_typ_norm_def
         (fun _ => True) (fun _ => True) (fun _ => True).
 
+    Ltac list_uninit_norm :=
+      intros ts Hts b;
+      rewrite Forall_forall in Hts;
+      specialize Hts with (b:=b);
+      rewrite <- Forall_forall in Hts;
+      apply map_ext_Forall in Hts;
+      do 2 f_equal; rewrite map_map; auto; assumption.
+
+    Ltac alist_uninit_norm :=
+      intros xts Hxts b;
+      rewrite Forall_forall in Hxts;
+      specialize Hxts with (b:=b);
+      rewrite <- Forall_forall in Hxts;
+      apply map_ext_Forall in Hxts;
+      do 2 f_equal;
+      rewrite <- map_map with
+          (g := uninit_sval_of_typ b) (f := snd) in Hxts;
+      rewrite <- map_map with
+          (g := uninit_sval_of_typ b) (f := fun xt => normᵗ (snd xt)) in Hxts;
+      rewrite <- map_map with
+          (g := normᵗ) (f := snd) in Hxts;
+      rewrite map_pat_combine, map_id;
+      unfold option_ret, option_bind;
+      induction xts as [| [[i x] t] xts IHxts];
+      simpl in *; inversion Hxts; subst; f_equal; auto; assumption.
+    
+    Lemma uninit_sval_of_typ_norm : forall t,
+        uninit_sval_of_typ_norm_def t.
+    Proof.
+      apply uninit_sval_of_typ_norm_ind;
+        unfold uninit_sval_of_typ_norm_def; cbn;
+          try (intros; f_equal; auto; assumption);
+          try list_uninit_norm; try alist_uninit_norm; auto.
+      - intros X [t |] [| m ms] H b; inversion H; subst; simpl in *; auto.
+    Qed.
+                                 
     Local Hint Constructors val_typ : core.
 
     Ltac some_inv :=
@@ -500,13 +616,16 @@ Section ValueTyping.
         |- _ => inversion H; subst; clear H
       end.
     
-    Lemma uninit_sval_of_typ_val_typ : forall t,
-        uninit_sval_of_typ_val_typ_def t.
+    Lemma uninit_sval_of_typ_val_typ : forall t b v ge,
+        is_expr_typ t ->
+        uninit_sval_of_typ b t = Some v ->
+        val_typ ge v (normᵗ t).
     Proof.
-      apply uninit_sval_of_typ_val_typ_ind;
-        unfold uninit_sval_of_typ_val_typ_def;
-        intros; cbn in *; try discriminate;
-          try some_inv; auto.
+      intros t b v ge H; generalize dependent ge;
+        generalize dependent v.
+      induction H using my_is_expr_typ_ind;
+        intros v ge Huninit; cbn in *;
+          try discriminate; try some_inv; auto.
       - assert (Hw : w = N.of_nat (length (repeat (@None bool) (N.to_nat w))))
           by (rewrite repeat_length; lia).
         rewrite Hw at 2; auto.
@@ -515,15 +634,16 @@ Section ValueTyping.
         rewrite Hw at 2; auto.
       - constructor; simpl; lia.
       - unfold option_bind, option_ret in *.
-        destruct (uninit_sval_of_typ b t) as [v' |] eqn:Hv';
-          cbn in *; try discriminate; some_inv.
+        destruct (uninit_sval_of_typ b (TypHeader ts))
+          as [v' |] eqn:Hv';
+          cbn in *; unfold option_bind, option_ret in *;
+            rewrite Hv' in Huninit; try discriminate.
+        apply IHis_expr_typ with (ge := ge) in Hv';
+          clear IHis_expr_typ; some_inv.
         assert (Hn : n = N.of_nat (length (repeat v' (N.to_nat n))))
           by (rewrite repeat_length; lia).
         rewrite Hn at 2.
-        Fail apply typ_stack.
-        admit. (* consider making [typ_stack] less restrictive,
-                  adding [is_expr] as an assumption &
-                  enforcing [TArray] there. *)
+        auto using Forall_repeat.
       - unfold option_bind, option_ret in *.
         destruct (sequence (map (uninit_sval_of_typ b) ts))
           as [vs |] eqn:Hvs; try discriminate; some_inv.
@@ -533,22 +653,36 @@ Section ValueTyping.
         apply Forall2_impl
           with (R := fun v t => uninit_sval_of_typ b t = Some v)
                (Q := val_typ ge); auto.
-        rewrite Forall2_forall.
-        rewrite Forall_forall in H.
-        split; eauto using Forall2_length.
-        intros v t HIn Huninit.
-        assert (HInts : List.In t ts) by admit.
-        (* TODO helper lemma for [combine]. *)
-        eauto.
+        + rewrite Forall2_forall.
+          rewrite Forall_forall in H0.
+          split.
+          * rewrite map_length. eauto using Forall2_length.
+          * intros u v HIn Hun.
+            apply in_combine_r in HIn.
+            rewrite in_map_iff in HIn.
+            destruct HIn as (t' & ? & Ht'); subst.
+            pose proof uninit_sval_of_typ_norm as Husotn;
+              unfold uninit_sval_of_typ_norm_def in Husotn;
+              rewrite Husotn in Hun; clear Husotn; eauto.
+        + admit.
       - unfold option_bind, option_ret in *.
         destruct (sequence (map (uninit_sval_of_typ b) ts))
           as [vs |] eqn:Hvs; try discriminate; some_inv.
         rewrite <- Forall2_sequence_iff,
         <- Forall2_map_l, Forall2_flip in Hvs.
-        Fail constructor.
+        constructor.
         admit. (* TODO: maybe need another constructor for [val_typ]. *)
       - admit.
       - admit.
+      - admit.
+      - admit.
+      - destruct t as [t |]; inversion H1; subst.
+        + apply H3 with (ge := ge) in Huninit. admit.
+        + assert (Hmems : PeanoNat.Nat.eqb (length mems) 0 = false)
+            by (rewrite PeanoNat.Nat.eqb_neq; lia).
+          rewrite Hmems in Huninit; some_inv.
+          destruct mems; simpl in *; try lia.
+          intuition.
     Admitted.
   End Uninit.
 End ValueTyping.
